Full proof that computeLeftSibling returns values needed on nextPath.

src/dafny/smart/PathInCompleteTrees.dfy
@@ -16,6 +16,7 @@ include "Trees2.dfy"
 include "CompleteTrees.dfy"
 include "SeqOfBits.dfy"
 include "Helpers.dfy"
+include "SeqHelpers.dfy"
 
 module PathInCompleteTrees {
 
@@ -23,6 +24,7 @@ module PathInCompleteTrees {
     import opened CompleteTrees
     import opened SeqOfBits
     import opened Helpers
+    import opened SeqHelpers
 
     /**
      *  The node at the end of a path.
@@ -475,8 +477,6 @@ module PathInCompleteTrees {
                     )
         )
     {
-       
-
         if |p| == 1 {
             //  Thanks Dafny
         } else {
@@ -542,18 +542,12 @@ module PathInCompleteTrees {
                         siblingAt(nextPath(p[.. |p| - 1])[..i + 1], r) == siblingAt(p[.. |p| - 1][..i + 1], r) 
                         );
                         assert(p[.. |p| - 1][..i + 1] == p[..i + 1]);
+                        assert(nextPath(p)[.. i + 1] == nextPath(p[.. |p| - 1 ])[..i + 1]);
 
                         assert(siblingAt(nextPath(p[.. |p| - 1 ])[..i + 1], r) == nodeAt(p[..i + 1], r)
                         ||
                         siblingAt(nextPath(p[.. |p| - 1])[..i + 1], r) == siblingAt(p[..i + 1], r) 
                         );
-                        // assert(exists i ::  0 <= i < |p[.. |p| - 1]| - 1  && p[.. |p| - 1][i] == 0 );
-
-                        // assert(
-                        //         siblingAt(nextPath(p[.. |p| - 1])[..i + 1],r) 
-                        //         == siblingAt(p[..i + 1], r));
-
-                        assume(siblingAt(nextPath(p)[..i + 1], r) == nodeAt(p[..i + 1], r));   
                     } else {
                         //  Thanks Dafny
                     }
@@ -567,4 +561,215 @@ module PathInCompleteTrees {
         ensures (s[.. |s| - 1] + [a])[..|s|] ==  s[.. |s| - 1] + [a]
     {}
 
+    function computeLeftSiblingOnNextPath <T>(p: seq<bit>, r : ITree<T>, v1 : seq<T>, v2 : seq<T>) : seq<T>
+        requires isCompleteTree(r)                              
+        requires 1 <= |p| <= height(r) - 1      
+        // requires 0 <= k < |nodesIn(r)|    - 1                     
+        // requires nodeAt(p, r) == nodesIn(r)[k]   
+        requires exists i :: 0 <= i < |p| && p[i] == 0
+        requires |v1| == |v2| == |p|
+        requires forall i :: 0 <= i < |p| ==>
+            v1[i] == nodeAt(p[.. i + 1],r).v 
+        requires forall i :: 0 <= i < |p| ==>
+            p[i] == 1 ==> v2[i] == siblingAt(p[.. i + 1],r).v 
+
+        ensures |computeLeftSiblingOnNextPath(p, r, v1, v2)| == |v1|
+        // ensures forall i :: 0 <= i < |p| ==>
+        //     nextPath(p)[i] == 1 ==> 
+        //         computeLeftSiblingOnNextPath(p, r, k, v1, v2)[i] == siblingAt(nextPath(p)[..i + 1],r).v
+    {
+        if |p| == 1 then
+            assert(p[0] == 0);
+                v1
+            // if p[|p| - 1] == 0 then 
+            //     //  Next path is p[..|p| - 1] + [1]
+            //     //  nextPath(p) and p agree on first |p| - 1 steps 
+            //     //  Collect values from v2[..|p| - 1 ] and add value at NodeAt(p,r)
+            //     v2[..|p| - 1] + [v1[|p| - 1 ]]
+            // else 
+        else 
+            assert(|p| >= 2);
+            if p[|p| - 1] == 0 then 
+                //  Next path is p[..|p| - 1] + [1]
+                //  nextPath(p) and p agree on first |p| - 1 steps 
+                //  Collect values from v2[..|p| - 1 ] and add value at NodeAt(p,r)
+                v2[..|p| - 1] + [v1[|p| - 1 ]]
+            else 
+                //  Nextpath is nextPath(p[.. |p| - 1]) + [0]
+                //  p[|p| - 1] == 0, next path will lead to another branch from ancestor
+                //  At that level in the tree nextPath(p)[|p| - 1] == 0 so whatever is good
+                // assert(exists i :: 0 <= i < |p| - 1 && p[i] == 0);
+                // assert(|v1[..|p| - 1]| == |v2[..|p| - 1]| == |p[.. |p| - 1]|);
+                // assert(forall i :: 0 <= i < |p| - 1 ==>
+                //         v1[i] == nodeAt(p[.. i + 1],r).v );
+
+                assert(forall i :: 0 <= i < |p| - 1 ==>
+                        p[.. i + 1] == p[..|p| - 1][.. i + 1]);
+
+                // assert(forall i :: 0 <= i < |p[..|p| - 1]|  ==>
+                        // v1[i] == nodeAt(p[..|p| - 1][.. i + 1],r).v );
+                // assert();
+                // assert(forall i :: 0 <= i < |p| ==>
+                //     p[i] == 1 ==> v2[i] == siblingAt(p[.. i + 1],r).v 
+                // );
+                computeLeftSiblingOnNextPath(p[.. |p| - 1], r, v1[..|p| - 1], v2[..|p| - 1]) + [v1[|p| - 1 ]]
+                // v1
+    } 
+
+    lemma foo500<T>(p: seq<bit>, r : ITree<T>, v1 : seq<T>, v2 : seq<T>)
+        requires isCompleteTree(r)                              
+        requires 1 <= |p| <= height(r) - 1      
+
+        requires exists i :: 0 <= i < |p| && p[i] == 0
+        requires |v1| == |v2| == |p|
+        requires forall i :: 0 <= i < |p| ==>
+            v1[i] == nodeAt(p[.. i + 1],r).v 
+        requires forall i :: 0 <= i < |p| ==>
+            p[i] == 1 ==> v2[i] == siblingAt(p[.. i + 1],r).v 
+
+        ensures forall i :: 0 <= i < |p| && nextPath(p)[i] == 1 ==> 
+                computeLeftSiblingOnNextPath(p, r, v1, v2)[i] == siblingAt(nextPath(p)[..i + 1],r).v
+    {    
+        if |p| == 1 {
+            forall (i : int |  0 <= i < |p| && nextPath(p)[i] == 1)
+                ensures computeLeftSiblingOnNextPath(p, r, v1, v2)[i] == siblingAt(nextPath(p)[..i + 1],r).v
+            {
+                //  i must be zero
+                assert(i == 0);
+                assert(siblingAt(nextPath(p)[..i + 1],r).v == nodeAt(p[.. i + 1],r).v) ;
+            }
+            // assert()
+        } else {
+            //  |p| >= 2
+            forall (i : int |  0 <= i < |p| && nextPath(p)[i] == 1)
+                ensures computeLeftSiblingOnNextPath(p, r, v1, v2)[i] == siblingAt(nextPath(p)[..i + 1],r).v
+            {
+                if (p[|p| - 1] == 0) {
+                    //  next path must end with 1 and hence p[|p| - 1] == 0
+                    assert(nextPath(p) == p[..|p| - 1] + [1]);
+                    assert(p[|p| - 1] == 0);
+                    if ( i < |p| - 1 ) {
+                        //  nextpath prefix is prefix of p
+                        calc {
+                            siblingAt(nextPath(p)[..i + 1],r).v ;
+                            == calc {
+                                nextPath(p)[..i + 1];
+                                ==
+                                p[.. i + 1];
+                            }
+                            siblingAt(p[.. i + 1], r).v ;
+                            ==
+                            v2[i];
+                            ==
+                            v2[..|p| - 1][i];
+                            == 
+                            (v2[..|p| - 1] + [v1[|p| - 1 ]])[i];
+                            ==
+                            computeLeftSiblingOnNextPath(p, r, v1, v2)[i];
+                        }
+                    
+                    } else {
+                        // i == |p| - 1
+                        calc {
+                            siblingAt(nextPath(p)[..i + 1],r).v ;
+                            == calc {
+                                i ;
+                                ==
+                                |p| - 1;
+                            }
+                            siblingAt(nextPath(p)[..|p|],r).v ;
+                            == { fullSliceIsSeq(nextPath(p)) ;}
+                            siblingAt(nextPath(p),r).v;
+                            == { foo900(p[..|p| - 1], r, 1); }
+                            nodeAt(p[..|p| - 1] + [0], r).v;
+                            == calc {
+                                p ;
+                                ==
+                                p[..|p| - 1] + [0];
+                            }
+                            nodeAt(p, r).v;
+                            == calc {
+                                p ;
+                                ==
+                                p[..|p| + 1 - 1];
+                            }
+                            nodeAt(p[.. |p| + 1 - 1],r).v;
+                            ==
+                            v1[|p| - 1];
+                            ==
+                            computeLeftSiblingOnNextPath(p, r, v1, v2)[|p| - 1] ;
+                            == calc {
+                                i ;
+                                ==
+                                |p| - 1;
+                            }
+                            computeLeftSiblingOnNextPath(p, r, v1, v2)[i] ;
+                        }
+                    }
+                } else {
+                    // p[|p| - 1] == 1
+                    assert(nextPath(p) == nextPath(p[.. |p| - 1]) + [0]);
+                    if ( i < |p| - 1 ) {
+                        assert(p[|p| - 1] == 1);
+                        //  Induction on p[.. |p| - 1]
+                        //  Check pre conditions to apply lemma inductively
+                       
+                        //  Requirement on v1
+                        forall (k : int | 0 <= k < |p[.. |p| - 1]| ) 
+                            ensures v1[k] == // nodeAt(p[.. k + 1],r).v == 
+                                          nodeAt(p[.. |p| - 1][.. k + 1],r).v
+                        {
+                            calc {
+                                v1[k];
+                                ==
+                                nodeAt(p[.. k + 1],r).v ;
+                                == calc {
+                                    p[.. |p| - 1][..k + 1] ;
+                                    ==
+                                    p[..k + 1];
+                                }
+                                nodeAt(p[.. |p| - 1][.. k + 1],r).v ;
+                            }
+                        }
+
+                        //  Requirement on v2
+                        forall (k : int | 0 <= k < |p[.. |p| - 1]| && p[.. |p| - 1][k] == 1 ) 
+                            ensures v2[k] == // nodeAt(p[.. k + 1],r).v == 
+                                          siblingAt(p[.. |p| - 1][.. k + 1],r).v
+                        {
+                            calc {
+                                v2[k];
+                                ==
+                                siblingAt(p[.. k + 1],r).v ;
+                                == calc {
+                                    p[.. |p| - 1][..k + 1] ;
+                                    ==
+                                    p[..k + 1];
+                                }
+                                siblingAt(p[.. |p| - 1][.. k + 1],r).v ;
+                            }
+                        }
+                        
+                        //  Induction hypothesis on p[.. |p| - 1], ... 
+                        foo500(p[.. |p| - 1], r, v1[..|p| - 1] , v2[..|p| - 1]);
+
+                        calc {
+                            computeLeftSiblingOnNextPath(p[..|p| - 1], r, v1[..|p| - 1], v2[..|p| - 1])[i] ;
+                            ==
+                            siblingAt(nextPath(p[..|p| - 1])[..i + 1],r).v;
+                            == calc {
+                                nextPath(p[..|p| - 1])[..i + 1];
+                                == 
+                                nextPath(p)[.. i + 1];
+                            }
+                            siblingAt(nextPath(p)[..i + 1],r).v;
+                        }
+                    } else {
+                        //  i == |p| - 1 and nextpath(p)[|p| - 1] == 0 so trivially true
+                        //  Thanks Dafny 
+                    }
+                }
+            }
+        }
+    }
 }
